\documentclass{amsart}


\DeclareMathOperator\erf{erf}
\DeclareMathOperator\erfinv{erfinv}
\begin{document}

\begin{equation}
\frac{d\log p(y_1, y_2, ..., y_n | A)}{dA} = \left( \sum_{i=1}^{n}\frac{1-y_i}{2} \right)  \frac{\frac{d}{dA} \Phi(\frac{-A}{\sigma})}{\Phi(\frac{-A}{\sigma})} - \left( \sum_{i=1}^{n}\frac{1+y_i}{2} \right)  \frac{\frac{d}{dA} \Phi(\frac{-A}{\sigma})}{1-\Phi(\frac{-A}{\sigma})}
\end{equation}

Where

\begin{equation}
\Phi(x) = \frac{1}{2} + \frac{1}{2}\erf(\frac{x}{\sqrt{2}})
\end{equation}

And

\begin{equation}
 \erf(x) = \frac{2}{\sqrt{\pi}} \int_{0}^{x}e^{-t^{2}}\, dt
\end{equation}

Note that

\begin{equation}
\frac{d}{dA}\Phi(\frac{-A}{\sigma}) = \frac{-1}{\sigma} \phi(\frac{-A}{\sigma})
\end{equation}

Where

\begin{equation}
\phi(x) = \frac{e^\frac{-x^2}{2}}{\sqrt{2\pi}}
\end{equation}

So this becomes

\begin{equation}
\frac{d\log p(y_1, y_2, ..., y_n | A)}{dA} = \left( \sum_{i=1}^{n}\frac{1-y_i}{2} \right)  \frac{\frac{-1}{\sigma} \phi(\frac{-A}{\sigma})}{\Phi(\frac{-A}{\sigma})} - \left( \sum_{i=1}^{n}\frac{1+y_i}{2} \right)  \frac{\frac{-1}{\sigma} \phi(\frac{-A}{\sigma})}{1-\Phi(\frac{-A}{\sigma})}
\end{equation}

Setting the derivative to 0 and simplifying, we get

\begin{equation}
\left( \sum_{i=1}^{n}\frac{1+y_i}{2} \right) \Phi(\frac{-A}{\sigma}) = \left( \sum_{i=1}^{n}\frac{1-y_i}{2} \right) \left( 1-\Phi(\frac{-A}{\sigma}) \right)
\end{equation}

Further simplifying

\begin{equation}
\Phi(\frac{-A}{\sigma}) = \frac{1}{n}\sum_{i=1}^{n}\frac{1-y_i}{2}
\end{equation}

So
\begin{equation}
A_{MLE} = -\sigma\Phi^{-1}\left(\frac{1}{n}\sum_{i=1}^{n}\frac{1-y_i}{2}\right)
\end{equation}


\newpage
Uniform Case:

\begin{equation}
\frac{d\log p(y_1, y_2, ..., y_n | A)}{dA} = \left(\sum_{i=1}^{n}\frac{1+y_i}{2}\right)\left( \frac{\sqrt{3}}{\sqrt{3}A + 3\sigma} \right) + \left(\sum_{i=1}^{n}\frac{1-y_i}{2}\right)\left( \frac{\sqrt{3}}{\sqrt{3}A - 3\sigma} \right)
\end{equation}

Setting the derivative to 0 and simplifying, we get

\begin{equation}
\sqrt{3}\sigma\left(\sum_{i=1}^{n}\frac{1+y_i}{2} - \sum_{i=1}^{n}\frac{1-y_i}{2}\right) = nA
\end{equation}

Which is the same as

\begin{equation}
\sqrt{3}\sigma\sum_{i=1}^{n}y_i = nA
\end{equation}

So

\begin{equation}
A_{MLE} = \frac{\sqrt{3}\sigma\sum_{i=1}^{n}y_i}{n} = \sqrt{3}\sigma\bar{y}
\end{equation}

\newpage

Gaussian MAP

By definition:

\begin{equation}
A_{MAP} = \max_{A} P(A|\underline{y}) = \max_{A}\frac{P(\underline{y}|A)P(A)}{P(\underline{y})}
\end{equation}

This is equivalent to 

\begin{equation}
A_{MAP} = \max_{A} \log P(A|\underline{y}) = \max_{A} \left( \log P(\underline{y}|A) + \log P(A) - \log P(\underline{y})\right)
\end{equation}

which is the same as 

\begin{equation}
A_{MAP} = \max_{A} \left( \log P(\underline{y}|A) + \log P(A)\right)
\end{equation}

In the Gaussian case, 

\begin{equation}
\log P(\underline{y}|A) = \left( \sum_{i=1}^{n}\frac{1-y_i}{2} \right) \log(1-\Phi(\frac{-A}{\sigma})) + \left( \sum_{i=1}^{n}\frac{1-y_i}{2} \right)  \log(\Phi(\frac{-A}{\sigma}))
\end{equation}

And

\begin{equation}
\log P(A) = \frac{-A^2}{2\sigma_{A}^2}
\end{equation}

So we define the MAP estimator as

\begin{equation}
A_{MAP} = \max_{A}\left( \left( \sum_{i=1}^{n}\frac{1-y_i}{2} \right) \log(1-\Phi(\frac{-A}{\sigma})) + \left( \sum_{i=1}^{n}\frac{1-y_i}{2} \right)  \log(\Phi(\frac{-A}{\sigma})) + \frac{-A^2}{2\sigma_{A}^2} \right)
\end{equation}

We solve this using MATLAB's fminunc function.

\newpage

Uniform MAP

Like in the Gaussian case, we define the conditional and marginal probabilities.

\begin{equation}
\log P(\underline{y}|A) = \left(\sum_{i=1}^{n}\frac{1+y_i}{2}\right)\log\left( \frac{1}{2} + \frac{A}{2\sqrt{3}\sigma} \right) + \left(\sum_{i=1}^{n}\frac{1-y_i}{2}\right)\log\left( \frac{1}{2} - \frac{A}{2\sqrt{3}\sigma} \right)
\end{equation}

\begin{equation}
\log P(A) = \log(\frac{-A + \sqrt{3}\sigma}{2\sqrt{3}\sigma})
\end{equation}

Following the definition of MAP,

\begin{equation}
A_{MAP} = \max_{A} \left( \left(\sum_{i=1}^{n}\frac{1+y_i}{2}\right)\log\left( \frac{1}{2} + \frac{A}{2\sqrt{3}\sigma} \right) + \left(\sum_{i=1}^{n}\frac{1-y_i}{2}\right)\log\left( \frac{1}{2} - \frac{A}{2\sqrt{3}\sigma} \right) + \log(\frac{-A + \sqrt{3}\sigma}{2\sqrt{3}\sigma}) \right)
\end{equation}

Again, we solve this using MATLAB's fminunc function


\newpage

Deriving MLE (Uniform Case)

\begin{equation}
\log P(\underline{y}|A) = \left(\sum_{i=1}^{n}\frac{1+y_i}{2}\right)\log\left( \frac{1}{2} + \frac{A}{2\sqrt{3}\sigma} \right) + \left(\sum_{i=1}^{n}\frac{1-y_i}{2}\right)\log\left( \frac{1}{2} - \frac{A}{2\sqrt{3}\sigma} \right)
\end{equation}

\begin{equation}
\frac{d\log p(\underline{y} | A)}{dA} = \left(\sum_{i=1}^{n}\frac{1+y_i}{2}\right)\left( \frac{\sqrt{3}}{\sqrt{3}A + 3\sigma} \right) + \left(\sum_{i=1}^{n}\frac{1-y_i}{2}\right)\left( \frac{\sqrt{3}}{\sqrt{3}A - 3\sigma} \right)
\end{equation}



\begin{equation}
0 = \frac{-\sum_{i=1}^{n} \frac{1-y_i}{2}}{-A+\sqrt{(3)\sigma}} + \frac{\sum_{i=1}^{n} \frac{1+y_i}{2}}{A+\sqrt{(3)\sigma}}
\end{equation}

\begin{equation}
\frac{\sum_{i=1}^{n} \frac{1-y_i}{2}}{-A+\sqrt{(3)\sigma}} = \frac{\sum_{i=1}^{n} \frac{1+y_i}{2}}{A+\sqrt{(3)\sigma}}
\end{equation}

\begin{equation}
(-A+\sqrt{3}\sigma)\sum_{i=1}^{n} \frac{1+y_i}{2} = (A+\sqrt{3}\sigma \sum_{i=1}^{n} \frac{1-y_i}{2})
\end{equation}

\begin{equation}
\sqrt{3}\left(\sigma\sum_{i=1}^{n} \frac{1+y_i}{2} - \sum_{i=1}^{n} \frac{1-y_i}{2}\right) = nA
\end{equation}

\begin{equation}
\sqrt{3}\sigma\sum_{i=1}^{n}y_i = nA
\end{equation}

\begin{equation}
A_{MLE} = \frac{\sqrt{3}\sigma\sum_{i=1}^{n}y_i}{n} = \sqrt{3}\sigma\bar{y}
\end{equation}

\newpage



Deriving MLE (Gaussian Case)

\begin{equation}
\log P(\underline{y}|A) = \left( \sum_{i=1}^{n}\frac{1-y_i}{2} \right) \log(1-\Phi(\frac{-A}{\sigma})) + \left( \sum_{i=1}^{n}\frac{1-y_i}{2} \right)  \log(\Phi(\frac{-A}{\sigma}))
\end{equation}

\begin{equation}
\frac{d\log p(\underline{y} | A)}{dA} = \left( \sum_{i=1}^{n}\frac{1-y_i}{2} \right)  \frac{\frac{d}{dA} \Phi(\frac{-A}{\sigma})}{\Phi(\frac{-A}{\sigma})} - \left( \sum_{i=1}^{n}\frac{1+y_i}{2} \right)  \frac{\frac{d}{dA} \Phi(\frac{-A}{\sigma})}{1-\Phi(\frac{-A}{\sigma})}
\end{equation}

\begin{equation}
\frac{d\log p(y_1, y_2, ..., y_n | A)}{dA} = \left( \sum_{i=1}^{n}\frac{1-y_i}{2} \right)  \frac{\frac{-1}{\sigma} \phi(\frac{-A}{\sigma})}{\Phi(\frac{-A}{\sigma})} - \left( \sum_{i=1}^{n}\frac{1+y_i}{2} \right)  \frac{\frac{-1}{\sigma} \phi(\frac{-A}{\sigma})}{1-\Phi(\frac{-A}{\sigma})}
\end{equation}

\begin{equation}
0 = \left( \sum_{i=1}^{n}\frac{1-y_i}{2} \right)  \frac{\frac{-1}{\sigma} \phi(\frac{-A}{\sigma})}{\Phi(\frac{-A}{\sigma})} - \left( \sum_{i=1}^{n}\frac{1+y_i}{2} \right)  \frac{\frac{-1}{\sigma} \phi(\frac{-A}{\sigma})}{1-\Phi(\frac{-A}{\sigma})}
\end{equation}

\begin{equation}
\left( \sum_{i=1}^{n}\frac{1+y_i}{2} \right)  \frac{\frac{-1}{\sigma} \phi(\frac{-A}{\sigma})}{1-\Phi(\frac{-A}{\sigma})} = 
\left( \sum_{i=1}^{n}\frac{1-y_i}{2} \right)  \frac{\frac{-1}{\sigma} \phi(\frac{-A}{\sigma})}{\Phi(\frac{-A}{\sigma})} 
\end{equation}

Cross multiplying, we get
\begin{equation}
\left(\sum_{i=1}^{n}\frac{1+y_i}{2}\right)\Phi(\frac{-A}{\sigma}) = \left(\sum_{i=1}^{n}\frac{1-y_i}{2}\right)\left(1-\Phi(\frac{-A}{\sigma})\right)
\end{equation}

\begin{equation}
\sum_{i=1}^{n}\frac{1-y_i}{2} = \Phi(\frac{-A}{\sigma})\left(\sum_{i=1}^{n}\frac{1+y_i}{2} + \sum_{i=1}^{n}\frac{1-y_i}{2}\right)
\end{equation}

\begin{equation}
\sum_{i=1}^{n}\frac{1-y_i}{2} = n\Phi(\frac{-A}{\sigma})
\end{equation}

\begin{equation}
\Phi(\frac{-A}{\sigma})= \frac{1}{n}\sum_{i=1}^{n}\frac{1-y_i}{2}
\end{equation}

\begin{equation}
A_{MLE} = -\sigma\Phi^{-1}\left(\frac{1}{n}\sum_{i=1}^{n}\frac{1-y_i}{2}\right)
\end{equation}

Where

\begin{equation}
\Phi^{-1}(x) = \sqrt{2}\erfinv(2x-1)
\end{equation}


\newpage

\end{document}


%------------------------------------------------------------------------------
% End of journal.tex
%------------------------------------------------------------------------------
